Prove that m is always greater than n at the beginning of step E1, except possibly the first time this step occurs.

m = qn + r for some integer q
After the first occurrence of E1, we know that n will either equal 0, or be the remainder of m divided by n.
In the case of r = 0, the algorithm terminates. In this case, m = qn. 

Therefore step 3 requires that: 1 <= r < n

In step 3:

    m <- n
    n <- r

Thus, the constraints mentioned earlier can be transformed to 1 <= n < m when step 1 is reached the second time.
